Define theorem 6.1

StaticScopes.v
@@ -21,10 +21,10 @@ Inductive DBExp : Set :=
     | DBVInt    : Z -> DBValue
     | DBVBool   : bool -> DBValue
     | DBVFun    : DBValueList -> DBExp -> DBValue
-    | DBVRecFun : DBValueList -> DBValue
+    | DBVRecFun : DBValueList -> DBExp -> DBValue
     with DBValueList : Set :=
-    | DVBLNil  : DBValueList
-    | DVBLCons : DBValueList -> DBValue -> DBValueList.
+    | DBVLNil  : DBValueList
+    | DBVLCons : DBValueList -> DBValue -> DBValueList.
 
 (* Variable list at p.97 *)
 Inductive VarList : Set :=
@@ -69,6 +69,101 @@ Inductive TransTo : VarList -> Exp -> DBExp -> Prop :=
                   TransTo (VLCons (VLCons X x) y) e1 d1 ->
                   TransTo (VLCons X x) e2 d2 ->
                   TransTo X (ELetRec x y e1 e2) (DBELetRec d1 d2).
+
+(* V[n] = w of at p.100 *)
+Inductive nth_val : DBValueList -> nat -> DBValue -> Prop :=
+    | NV_O : forall w : DBValue, nth_val (DBVLCons DBVLNil w) O w
+    | NV_S : forall (V : DBValueList) (n : nat) (w w0 : DBValue),
+             nth_val V n w ->
+             nth_val (DBVLCons V w0) (S n) w.
+
+(* Fig 6.3, 6.4 *)
+Inductive DBEvalTo : DBValueList -> DBExp -> DBValue -> Prop :=
+    | DBE_Int    : forall (V : DBValueList) (i : Z),
+                   DBEvalTo V (DBEValue (DBVInt i)) (DBVInt i)
+    | DBE_Bool   : forall (V : DBValueList) (b : bool),
+                   DBEvalTo V (DBEValue (DBVBool b)) (DBVBool b)
+    | DBE_IfT    : forall (V : DBValueList) (d1 d2 d3 : DBExp) (w : DBValue),
+                   DBEvalTo V d1 (DBVBool true) -> DBEvalTo V d2 w ->
+                   DBEvalTo V (DBEIf d1 d2 d3) w
+    | DBE_IfF    : forall (V : DBValueList) (d1 d2 d3 : DBExp) (w : DBValue),
+                   DBEvalTo V d1 (DBVBool false) -> DBEvalTo V d3 w ->
+                   DBEvalTo V (DBEIf d1 d2 d3) w
+    | DBE_Plus   : forall (V : DBValueList) (d1 d2 d3 : DBExp) (i1 i2 i3 : Z),
+                   DBEvalTo V d1 (DBVInt i1) -> DBEvalTo V d2 (DBVInt i2) ->
+                   Plus i1 i2 i3 ->
+                   DBEvalTo V (DBEPlus d1 d2) (DBVInt i3)
+    | DBE_Minus  : forall (V : DBValueList) (d1 d2 d3 : DBExp) (i1 i2 i3 : Z),
+                   DBEvalTo V d1 (DBVInt i1) -> DBEvalTo V d2 (DBVInt i2) ->
+                   Minus i1 i2 i3 ->
+                   DBEvalTo V (DBEMinus d1 d2) (DBVInt i3)
+    | DBE_Times  : forall (V : DBValueList) (d1 d2 d3 : DBExp) (i1 i2 i3 : Z),
+                   DBEvalTo V d1 (DBVInt i1) -> DBEvalTo V d2 (DBVInt i2) ->
+                   Times i1 i2 i3 ->
+                   DBEvalTo V (DBETimes d1 d2) (DBVInt i3)
+    | DBE_Lt     : forall (V : DBValueList) (d1 d2 d3 : DBExp)
+                          (i1 i2 : Z) (b3 : bool),
+                   DBEvalTo V d1 (DBVInt i1) -> DBEvalTo V d2 (DBVInt i2) ->
+                   Lt i1 i2 b3 ->
+                   DBEvalTo V (DBELt d1 d2) (DBVBool b3)
+    | DBE_Var    : forall (V : DBValueList) (n : nat) (w : DBValue),
+                   nth_val V n w ->
+                   DBEvalTo V (DBEVar n) w
+    | DBE_Let    : forall (V : DBValueList) (d1 d2 : DBExp) (w w1 : DBValue),
+                   DBEvalTo V d1 w1 -> DBEvalTo (DBVLCons V w1) d2 w ->
+                   DBEvalTo V (DBELet d1 d2) w
+    | DBE_Fun    : forall (V : DBValueList) (d : DBExp),
+                   DBEvalTo V (DBEFun d) (DBVFun V d)
+    | DBE_App    : forall (V V2 : DBValueList) (d1 d2 d0 : DBExp)
+                          (w w2 : DBValue),
+                   DBEvalTo V d1 (DBVFun V2 d0) -> DBEvalTo V d2 w2 ->
+                   DBEvalTo (DBVLCons V2 w2) d0 w ->
+                   DBEvalTo V (DBEApp d1 d2) w
+    | DBE_LetRec : forall (V : DBValueList) (d1 d2 : DBExp) (w : DBValue),
+                   DBEvalTo (DBVLCons V (DBVRecFun V d1)) d2 w ->
+                   DBEvalTo V (DBELetRec d1 d2) w
+    | DBE_AppRec : forall (V V2 : DBValueList) (d1 d2 d0 : DBExp)
+                          (w w2 : DBValue),
+                   DBEvalTo V d2 (DBVRecFun V2 d0) -> DBEvalTo V d2 w2 ->
+                   DBEvalTo (DBVLCons (DBVLCons V2 (DBVRecFun V2 d0)) w2) d0 w ->
+                   DBEvalTo V (DBEApp d1 d2) w.
+
+(* Fig 6.5 *)
+Inductive TransValTo : Value -> DBValue -> Prop :=
+    | Trv_Int  : forall i : Z, TransValTo (VInt i) (DBVInt i)
+    | Trv_Bool : forall b : bool, TransValTo (VBool b) (DBVBool b)
+    | Trv_Fun  : forall (E : Env) (X : VarList) (V : DBValueList) (x : Var)
+                        (e : Exp) (d : DBExp),
+                 TransEnvTo E X V -> TransTo (VLCons X x) e d ->
+                 TransValTo (VFun E x e) (DBVFun V d)
+    | Trv_Rec  : forall (E : Env) (X : VarList) (V : DBValueList) (x y : Var)
+                        (e : Exp) (d : DBExp),
+                 TransEnvTo E X V -> TransTo (VLCons (VLCons X x) y) e d ->
+                 TransValTo (VRecFun E x y e) (DBVRecFun V d)
+    with TransEnvTo : Env -> VarList -> DBValueList -> Prop :=
+    | Tre_Empty : TransEnvTo ENil VLNil DBVLNil
+    | Tre_Bind  : forall (E : Env) (X : VarList) (V : DBValueList)
+                         (x : Var) (v : Value) (w : DBValue),
+                  TransEnvTo E X V -> TransValTo v w ->
+                  TransEnvTo (ECons E x v) (VLCons X x) (DBVLCons V w).
+
+(* Theorem 6.1 (1) *)
+Theorem EvalTo_DBEvalTo_compat :
+    forall (E : Env) (X : VarList) (V : DBValueList)
+           (e : Exp) (d : DBExp) (v : Value),
+    TransEnvTo E X V -> TransTo X e d -> EvalTo E e v ->
+    exists w : DBValue, (DBEvalTo V d w /\ TransValTo v w).
+Proof.
+Admitted.
+
+(* Theorem 6.1 (2) *)
+Theorem DBEvalTo_EvalTo_compat :
+    forall (E : Env) (X : VarList) (V : DBValueList)
+           (e : Exp) (d : DBExp) (w : DBValue),
+    TransEnvTo E X V -> TransTo X e d -> DBEvalTo V d w ->
+    exists v : Value, (EvalTo E e v /\ TransValTo v w).
+Proof.
+Admitted.
 
 End StaticScopes.
 
